Specify operations

theories/Circuit.v
@@ -1,7 +1,6 @@
 Require Import Utils.
 
 Require Import Lia.
-
 Require Coq.Lists.List.
 Import List.ListNotations.
 Import Coq.NArith.BinNat.
@@ -55,8 +54,6 @@ Definition reference_wf input_count wire_count r :=
   | reference_Wire i => (i < wire_count)%N
   end.
 
-Register reference_wf as vcpu.reference.wf.
-
 Definition binding_wf input_count wire_count b :=
   match b with
   | binding_Immidiate r => reference_wf input_count wire_count r
@@ -76,6 +73,7 @@ Definition binding_wf input_count wire_count b :=
     reference_wf input_count wire_count r3
   end.
 
+Register reference_wf as vcpu.reference.wf.
 Register binding_wf as vcpu.binding.wf.
 
 Definition reference_wf_b input_count wire_count r :=
@@ -122,7 +120,7 @@ Proof.
 Qed.
 
 Definition circuit_wire_count_wf c :=
-  N.of_nat (length (circuit_wires c)) = circuit_wire_count c.
+  length_bin (circuit_wires c) = circuit_wire_count c.
 
 Definition circuit_wires_wf c :=
   list_forall_i_bin (binding_wf (circuit_input_count c)) (circuit_wires c).
@@ -174,8 +172,8 @@ Definition reference_compute inputs intermediates r :=
   match r with
   | reference_Zero => false
   | reference_One => true
-  | reference_Input i => List.nth (N.to_nat i) inputs false
-  | reference_Wire i => List.nth (N.to_nat i) intermediates false
+  | reference_Input i => list_nth_bin i inputs false
+  | reference_Wire i => list_nth_bin i intermediates false
   end.
 
 Definition binding_compute inputs intermediates b :=
@@ -205,14 +203,40 @@ Definition circuit_compute_wires c inputs :=
 Definition circuit_compute c inputs :=
   list_select_bin (circuit_compute_wires c inputs) (circuit_outputs c) false.
 
+Theorem length_bin_circuit_compute_wires_aux :
+  forall start_intermediates wires inputs,
+  length_bin (circuit_compute_wires_aux start_intermediates wires inputs) = length_bin wires.
+Proof.
+  intros start_intermediates wires inputs. unfold circuit_compute_wires_aux.
+  cut (
+    forall l,
+    length_bin (List.fold_left (fun intermediates b =>
+      intermediates ++ [binding_compute inputs (start_intermediates ++ intermediates) b]
+    ) wires l) = (length_bin l + length_bin wires)%N
+  ).
+  - intros H. apply (H []).
+  - induction wires as [ | b wires' IH]; intros l.
+    + simpl. rewrite length_bin_nil. lia.
+    + simpl. rewrite IH. rewrite length_bin_app, ? length_bin_cons, length_bin_nil. lia.
+Qed.
+
+Lemma circuit_compute_wires_aux_app :
+  forall start_intermediates wires_1 wires_2 inputs,
+  circuit_compute_wires_aux start_intermediates (wires_1 ++ wires_2) inputs =
+    let intermediates_1 := circuit_compute_wires_aux start_intermediates wires_1 inputs in
+    intermediates_1 ++ circuit_compute_wires_aux (start_intermediates ++ intermediates_1) wires_2 inputs.
+Proof.
+  intros start_intermediates wires_1 wires_2 inputs. simpl. unfold circuit_compute_wires_aux.
+  rewrite List.fold_left_app. rewrite list_fold_left_app_shift. f_equal. apply list_fold_left_ext.
+  intros intermediates b. rewrite List.app_assoc. auto.
+Qed.
+
 Definition circuit_set_outputs c outputs := {|
   circuit_input_count := circuit_input_count c;
   circuit_wire_count := circuit_wire_count c;
   circuit_wires := circuit_wires c;
   circuit_outputs := outputs;
 |}.
-
-Register circuit_set_outputs as vcpu.circuit.set_outputs.
 
 Lemma circuit_set_outputs_wf :
   forall c outputs,
@@ -226,7 +250,15 @@ Proof.
   - apply H2.
 Qed.
 
-Register circuit_set_outputs_wf as vcpu.circuit.set_outputs_wf.
+Lemma circuit_set_outputs_spec_wires :
+  forall c outputs,
+  circuit_wf c ->
+  list_forall (fun i => (i < circuit_wire_count c)%N) outputs ->
+  forall inputs, length_bin inputs = circuit_input_count c ->
+  circuit_compute_wires (circuit_set_outputs c outputs) inputs = circuit_compute_wires c inputs.
+Proof.
+  intros c outputs H1 H2 inputs H3. unfold circuit_compute_wires. auto.
+Qed.
 
 Definition circuit_set_outputs_with_wf
   c_with_wf outputs
@@ -252,7 +284,7 @@ Definition circuit_add_translate_reference parent_wire_count input_references r 
   match r with
   | reference_Zero => reference_Zero
   | reference_One => reference_One
-  | reference_Input i => List.nth (N.to_nat i) input_references reference_Zero
+  | reference_Input i => list_nth_bin i input_references reference_Zero
   | reference_Wire i => reference_Wire (parent_wire_count + i)
   end.
 
@@ -278,13 +310,11 @@ Definition circuit_add c_parent c_child input_references := {|
   circuit_outputs := circuit_outputs c_parent;
 |}.
 
-Register circuit_add as vcpu.circuit.add.
-
 Lemma circuit_add_translate_reference_wf :
   forall c_parent c_child input_references,
   circuit_wf c_parent ->
   circuit_wf c_child ->
-  N.of_nat (length input_references) = circuit_input_count c_child ->
+  length_bin input_references = circuit_input_count c_child ->
   list_forall
     (reference_wf (circuit_input_count c_parent) (circuit_wire_count c_parent))
     input_references ->
@@ -299,7 +329,7 @@ Proof.
   destruct r as [ | | j | j]; simpl; simpl in H5.
   - auto.
   - auto.
-  - apply list_forall_list_nth.
+  - apply list_forall_list_nth_bin.
     + apply (list_forall_incr _ _ _ H4). intros r H6. apply (reference_wf_big_enough _ _ _ _ _ H6); lia.
     + lia.
   - lia.
@@ -309,7 +339,7 @@ Lemma circuit_add_translate_binding_wf :
   forall c_parent c_child input_references,
   circuit_wf c_parent ->
   circuit_wf c_child ->
-  N.of_nat (length input_references) = circuit_input_count c_child ->
+  length_bin input_references = circuit_input_count c_child ->
   list_forall
     (reference_wf (circuit_input_count c_parent) (circuit_wire_count c_parent))
     input_references ->
@@ -329,15 +359,15 @@ Lemma circuit_add_wf :
   forall c_parent c_child input_references,
   circuit_wf c_parent ->
   circuit_wf c_child ->
-  N.of_nat (length input_references) = circuit_input_count c_child ->
+  length_bin input_references = circuit_input_count c_child ->
   list_forall
     (reference_wf (circuit_input_count c_parent) (circuit_wire_count c_parent))
     input_references ->
   circuit_wf (circuit_add c_parent c_child input_references).
 Proof.
   intros c_parent c_child input_references H1 H2 H3. repeat split.
-  - unfold circuit_wire_count_wf. simpl. rewrite List.app_length. rewrite List.map_length.
-    rewrite Nnat.Nat2N.inj_add. rewrite (proj1 H1), (proj1 H2). auto.
+  - unfold circuit_wire_count_wf. simpl. rewrite length_bin_app. rewrite length_bin_list_map.
+    rewrite (proj1 H1), (proj1 H2). auto.
   - unfold circuit_wires_wf. simpl. rewrite list_forall_i_bin_app. rewrite (proj1 H1). split.
     + apply (proj1 (proj2 H1)).
     + rewrite list_forall_i_bin_aux_map. rewrite list_forall_i_bin_aux_to_simple.
@@ -347,11 +377,89 @@ Proof.
     simpl. lia.
 Qed.
 
-Register circuit_add_wf as vcpu.circuit.add_wf.
+Lemma circuit_add_translate_reference_spec :
+  forall c_parent c_child input_references,
+  circuit_wf c_parent ->
+  circuit_wf c_child ->
+  length_bin input_references = circuit_input_count c_child ->
+  list_forall
+    (reference_wf (circuit_input_count c_parent) (circuit_wire_count c_parent))
+    input_references ->
+  forall inputs, length_bin inputs = circuit_input_count c_parent ->
+  let parent_intermediates := circuit_compute_wires c_parent inputs in
+  forall intermediates i r,
+  reference_wf (circuit_input_count c_child) i r ->
+  reference_compute inputs (parent_intermediates ++ intermediates)
+    (circuit_add_translate_reference (circuit_wire_count c_parent) input_references r) =
+  reference_compute (List.map (reference_compute inputs parent_intermediates) input_references) intermediates r.
+Proof.
+  intros c_parent c_child input_references H1 H2 H3 H4 inputs H5 parent_intermediates intermediates i r H6.
+  assert (H7 : length_bin parent_intermediates = circuit_wire_count c_parent). {
+    subst parent_intermediates. unfold circuit_compute_wires. rewrite length_bin_circuit_compute_wires_aux.
+    rewrite (proj1 H1). auto.
+  }
+  destruct r as [ | | j | j]; simpl.
+  - auto.
+  - auto.
+  - replace false with (reference_compute inputs parent_intermediates reference_Zero) by auto.
+    rewrite list_nth_bin_list_map. remember (list_nth_bin j input_references reference_Zero) as r eqn:Heqr.
+    destruct r as [ | | k | k]; simpl.
+    + auto.
+    + auto.
+    + auto.
+    + apply list_app_bin_nth_1. simpl in H6. rewrite <- H3 in H6.
+      specialize (list_forall_list_nth_bin _ _ _ reference_Zero H4 H6) as H8. rewrite <- Heqr in H8. simpl in H8.
+      lia.
+  - replace (circuit_wire_count c_parent) with (length_bin parent_intermediates). apply list_app_bin_nth_2_add.
+Qed.
+
+Lemma circuit_add_translate_binding_spec :
+  forall c_parent c_child input_references,
+  circuit_wf c_parent ->
+  circuit_wf c_child ->
+  length_bin input_references = circuit_input_count c_child ->
+  list_forall
+    (reference_wf (circuit_input_count c_parent) (circuit_wire_count c_parent))
+    input_references ->
+  forall inputs, length_bin inputs = circuit_input_count c_parent ->
+  let parent_intermediates := circuit_compute_wires c_parent inputs in
+  forall intermediates i b,
+  binding_wf (circuit_input_count c_child) i b ->
+  binding_compute inputs (parent_intermediates ++ intermediates)
+    (circuit_add_translate_binding (circuit_wire_count c_parent) input_references b) =
+  binding_compute (List.map (reference_compute inputs parent_intermediates) input_references) intermediates b.
+Proof.
+  intros c_parent c_child input_references H1 H2 H3 H4 inputs H5 parent_intermediates intermediates i b H6.
+  destruct b as [r | r | r1 r2 | r1 r2 | r1 r2 | r1 r2 r3]; simpl; simpl in H6;
+  rewrite ? (circuit_add_translate_reference_spec _ _ _ H1 H2 H3 H4 _ H5 _ i); intuition auto.
+Qed.
+
+Lemma circuit_add_spec_wires :
+  forall c_parent c_child input_references,
+  circuit_wf c_parent ->
+  circuit_wf c_child ->
+  length_bin input_references = circuit_input_count c_child ->
+  list_forall
+    (reference_wf (circuit_input_count c_parent) (circuit_wire_count c_parent))
+    input_references ->
+  forall inputs, length_bin inputs = circuit_input_count c_parent ->
+  let parent_intermediates := circuit_compute_wires c_parent inputs in
+  let child_inputs := List.map (reference_compute inputs parent_intermediates) input_references in
+  circuit_compute_wires (circuit_add c_parent c_child input_references) inputs =
+    parent_intermediates ++ circuit_compute_wires c_child child_inputs.
+Proof.
+  intros c_parent c_child input_references H1 H2 H3 H4 inputs H5 parent_intermediates child_inputs.
+  unfold circuit_compute_wires, circuit_add. simpl. rewrite circuit_compute_wires_aux_app.
+  replace (circuit_compute_wires_aux [] (circuit_wires c_parent) inputs) with parent_intermediates by auto.
+  simpl. f_equal. subst child_inputs. unfold circuit_compute_wires_aux.
+  rewrite list_fold_left_list_map. apply list_fold_left_ext_precise. intros intermediates.
+  rewrite list_forall_list_forall_i_bin. apply (list_forall_i_bin_incr _ _ _ (proj1 (proj2 H2))).
+  intros i b H6. do 2 f_equal. apply (circuit_add_translate_binding_spec _ _ _ H1 H2 H3 H4 _ H5 _ _ _ H6).
+Qed.
 
 Definition circuit_add_with_wf
   c_parent_with_wf c_child_with_wf input_references
-  (H1 : N.of_nat (length input_references) = circuit_input_count (circuit_with_wf_circuit c_child_with_wf))
+  (H1 : length_bin input_references = circuit_input_count (circuit_with_wf_circuit c_child_with_wf))
   (H2 :
     list_forall_b
       (
@@ -385,16 +493,12 @@ Definition circuit_empty input_count := {|
   circuit_outputs := [];
 |}.
 
-Register circuit_empty as vcpu.circuit.empty.
-
 Theorem circuit_empty_wf :
   forall input_count,
   circuit_wf (circuit_empty input_count).
 Proof.
   intros input_count. cbv. auto.
 Qed.
-
-Register circuit_empty_wf as vcpu.circuit.empty_wf.
 
 Definition circuit_empty_with_wf input_count : circuit_with_wf := {|
   circuit_with_wf_circuit := circuit_empty input_count;
@@ -406,23 +510,43 @@ Register circuit_empty_with_wf as vcpu.circuit.empty_with_wf.
 Definition circuit_id input_count := {|
   circuit_input_count := input_count;
   circuit_wire_count := input_count;
-  circuit_wires := list_init (fun i => binding_Immidiate (reference_Input (N.of_nat i))) (N.to_nat input_count);
-  circuit_outputs := List.map N.of_nat (List.seq 0 (N.to_nat input_count));
+  circuit_wires := list_init_bin (fun i => binding_Immidiate (reference_Input i)) input_count;
+  circuit_outputs := list_seq_bin 0 input_count;
 |}.
-
-Register circuit_id as vcpu.circuit.id.
 
 Theorem circuit_id_wf :
   forall input_count,
   circuit_wf (circuit_id input_count).
 Proof.
   intros input_count. repeat split.
-  - unfold circuit_wire_count_wf. simpl. rewrite length_list_init. lia.
-  - unfold circuit_wires_wf. simpl. rewrite list_forall_i_bin_equiv. rewrite list_forall_i_list_init. simpl. lia.
-  - unfold circuit_outputs_wf. simpl. rewrite list_forall_list_map. rewrite list_forall_list_seq. simpl. lia.
+  - unfold circuit_wire_count_wf. simpl. apply length_bin_list_init_bin.
+  - unfold circuit_wires_wf. simpl. rewrite list_forall_i_bin_list_init_bin. simpl. auto.
+  - unfold circuit_outputs_wf. simpl. apply list_forall_list_seq_bin. auto.
 Qed.
 
-Register circuit_id_wf as vcpu.circuit.id_wf.
+Lemma circuit_id_spec_wires :
+  forall input_count,
+  forall inputs, length_bin inputs = input_count ->
+  circuit_compute_wires (circuit_id input_count) inputs = inputs.
+Proof.
+  intros input_count inputs H. unfold circuit_compute_wires, circuit_compute_wires_aux, circuit_id. simpl.
+  rewrite list_fold_left_list_init_bin. rewrite <- H; clear input_count H.
+  - induction inputs as [ | x inputs' IH].
+    + auto.
+    + simpl. rewrite length_bin_cons. rewrite list_seq_bin_succ. simpl. rewrite list_fold_left_app_shift. simpl.
+      f_equal. rewrite (list_fold_left_list_seq_bin_shift _ 0 1). rewrite <- IH at 2. simpl.
+      apply list_fold_left_ext. intros intermediates i. rewrite <- succ_to_add. rewrite list_nth_bin_succ_cons.
+      auto.
+Qed.
+
+Lemma circuit_id_spec :
+  forall input_count,
+  forall inputs, length_bin inputs = input_count ->
+  circuit_compute (circuit_id input_count) inputs = inputs.
+Proof.
+  intros input_count inputs H. unfold circuit_compute. rewrite (circuit_id_spec_wires _ _ H). simpl.
+  rewrite <- H. apply list_select_bin_all.
+Qed.
 
 Definition circuit_id_with_wf input_count : circuit_with_wf := {|
   circuit_with_wf_circuit := circuit_id input_count;
@@ -438,15 +562,11 @@ Definition circuit_zero := {|
   circuit_outputs := [0%N];
 |}.
 
-Register circuit_zero as vcpu.circuit.zero.
-
 Theorem circuit_zero_wf :
   circuit_wf circuit_zero.
 Proof.
   cbv. auto.
 Qed.
-
-Register circuit_zero_wf as vcpu.circuit.zero_wf.
 
 Definition circuit_zero_with_wf : circuit_with_wf := {|
   circuit_with_wf_circuit := circuit_zero;
@@ -462,15 +582,11 @@ Definition circuit_one := {|
   circuit_outputs := [0%N];
 |}.
 
-Register circuit_one as vcpu.circuit.one.
-
 Theorem circuit_one_wf :
   circuit_wf circuit_one.
 Proof.
   cbv. auto.
 Qed.
-
-Register circuit_one_wf as vcpu.circuit.one_wf.
 
 Definition circuit_one_with_wf : circuit_with_wf := {|
   circuit_with_wf_circuit := circuit_one;
@@ -486,15 +602,11 @@ Definition circuit_not := {|
   circuit_outputs := [0%N];
 |}.
 
-Register circuit_not as vcpu.circuit.not.
-
 Theorem circuit_not_wf :
   circuit_wf circuit_not.
 Proof.
   cbv. auto.
 Qed.
-
-Register circuit_not_wf as vcpu.circuit.not_wf.
 
 Definition circuit_not_with_wf : circuit_with_wf := {|
   circuit_with_wf_circuit := circuit_not;
@@ -510,15 +622,11 @@ Definition circuit_and := {|
   circuit_outputs := [0%N];
 |}.
 
-Register circuit_and as vcpu.circuit.and.
-
 Theorem circuit_and_wf :
   circuit_wf circuit_and.
 Proof.
   cbv. auto.
 Qed.
-
-Register circuit_and_wf as vcpu.circuit.and_wf.
 
 Definition circuit_and_with_wf : circuit_with_wf := {|
   circuit_with_wf_circuit := circuit_and;
@@ -534,15 +642,11 @@ Definition circuit_or := {|
   circuit_outputs := [0%N];
 |}.
 
-Register circuit_or as vcpu.circuit.or.
-
 Theorem circuit_or_wf :
   circuit_wf circuit_or.
 Proof.
   cbv. auto.
 Qed.
-
-Register circuit_or_wf as vcpu.circuit.or_wf.
 
 Definition circuit_or_with_wf : circuit_with_wf := {|
   circuit_with_wf_circuit := circuit_or;
@@ -558,15 +662,11 @@ Definition circuit_xor := {|
   circuit_outputs := [0%N];
 |}.
 
-Register circuit_xor as vcpu.circuit.xor.
-
 Theorem circuit_xor_wf :
   circuit_wf circuit_xor.
 Proof.
   cbv. auto.
 Qed.
-
-Register circuit_xor_wf as vcpu.circuit.xor_wf.
 
 Definition circuit_xor_with_wf : circuit_with_wf := {|
   circuit_with_wf_circuit := circuit_xor;
@@ -579,28 +679,57 @@ Definition circuit_switch data_size := {|
   circuit_input_count := 1 + 2 * data_size;
   circuit_wire_count := data_size;
   circuit_wires :=
-    list_init (fun i =>
+    list_init_bin (fun i =>
       binding_If
         (reference_Input 0)
-        (reference_Input (1 + N.of_nat i))
-        (reference_Input (1 + data_size + N.of_nat i))
-    ) (N.to_nat data_size);
-  circuit_outputs := List.map N.of_nat (List.seq 0 (N.to_nat data_size));
+        (reference_Input (1 + i))
+        (reference_Input (1 + data_size + i))
+    ) data_size;
+  circuit_outputs := list_seq_bin 0 data_size;
 |}.
-
-Register circuit_switch as vcpu.circuit.switch.
 
 Theorem circuit_switch_wf :
   forall data_size,
   circuit_wf (circuit_switch data_size).
 Proof.
   intros data_size. repeat split.
-  - unfold circuit_wire_count_wf. simpl. rewrite length_list_init. lia.
-  - unfold circuit_wires_wf. rewrite list_forall_i_bin_equiv. simpl. rewrite list_forall_i_list_init. simpl. lia.
-  - unfold circuit_outputs_wf. simpl. rewrite list_forall_list_map. rewrite list_forall_list_seq. lia.
+  - unfold circuit_wire_count_wf. simpl. apply length_bin_list_init_bin.
+  - unfold circuit_wires_wf. simpl. rewrite list_forall_i_bin_list_init_bin. simpl. lia.
+  - unfold circuit_outputs_wf. simpl. rewrite list_forall_list_seq_bin. auto.
 Qed.
 
-Register circuit_switch_wf as vcpu.circuit.switch_wf.
+Lemma circuit_switch_spec_wires :
+  forall data_size,
+  forall inputs, length_bin inputs = (1 + 2 * data_size)%N ->
+  circuit_compute_wires (circuit_switch data_size) inputs =
+    if list_nth_bin 0 inputs false
+    then list_select_bin inputs (list_seq_bin (1 + data_size) data_size) false
+    else list_select_bin inputs (list_seq_bin 1 data_size) false.
+Proof.
+  intros data_size inputs H. unfold circuit_compute_wires, circuit_compute_wires_aux, circuit_switch. simpl.
+  rewrite list_fold_left_list_init_bin. simpl. rewrite <- list_map_list_fold_left. unfold list_select_bin.
+  destruct (list_nth_bin 0 inputs false).
+  - rewrite (list_seq_bin_to_simple (1 + data_size)). rewrite List.map_map. auto.
+  - rewrite (list_seq_bin_to_simple 1). rewrite List.map_map. auto.
+Qed.
+
+Lemma circuit_switch_spec :
+  forall data_size,
+  forall inputs, length_bin inputs = (1 + 2 * data_size)%N ->
+  circuit_compute (circuit_switch data_size) inputs =
+    if list_nth_bin 0 inputs false
+    then list_select_bin inputs (list_seq_bin (1 + data_size) data_size) false
+    else list_select_bin inputs (list_seq_bin 1 data_size) false.
+Proof.
+  intros data_size inputs H. unfold circuit_compute. rewrite (circuit_switch_spec_wires _ _ H). simpl.
+  replace data_size with (length_bin (if list_nth_bin 0 inputs false
+      then list_select_bin inputs (list_seq_bin (1 + data_size) data_size) false
+      else list_select_bin inputs (list_seq_bin 1 data_size) false)) at 4.
+  - apply list_select_bin_all.
+  - destruct (list_nth_bin 0 inputs false).
+    + rewrite length_bin_list_select_bin. apply length_list_seq_bin.
+    + rewrite length_bin_list_select_bin. apply length_list_seq_bin.
+Qed.
 
 Definition circuit_switch_with_wf data_size : circuit_with_wf := {|
   circuit_with_wf_circuit := circuit_switch data_size;
@@ -609,12 +738,12 @@ Definition circuit_switch_with_wf data_size : circuit_with_wf := {|
 
 Register circuit_switch_with_wf as vcpu.circuit.switch_with_wf.
 
-(*Definition circuit_simplify_translate_reference mapping r :=
+Definition circuit_simplify_translate_reference mapping r :=
   match r with
   | reference_Zero => reference_Zero
   | reference_One => reference_One
   | reference_Input i => reference_Input i
-  | reference_Wire i => reference_Wire (nat_list_assoc i mapping 0)
+  | reference_Wire i => reference_Wire (binnat_list_assoc i mapping 0%N)
   end.
 
 Definition circuit_simplify_translate_binding mapping b :=
@@ -634,609 +763,23 @@ Definition circuit_simplify c :=
       match b with
       | binding_Immidiate (reference_Wire j) =>
         (
-          S i,
+          N.succ i,
           wires,
-          mapping ++ [(i, nat_list_assoc j mapping 0)]
+          mapping ++ [(i, binnat_list_assoc j mapping 0%N)]
         )
       | _ =>
         (
-          S i,
+          N.succ i,
           wires ++ [circuit_simplify_translate_binding mapping b],
-          mapping ++ [(i, length wires)]
+          mapping ++ [(i, length_bin wires)]
         )
       end
-    ) (circuit_wires c) (0, [], []) in
+    ) (circuit_wires c) (0%N, [], []) in
   {|
     circuit_input_count := circuit_input_count c;
+    circuit_wire_count := length_bin wires;
     circuit_wires := wires;
-    circuit_outputs := List.map (fun i => nat_list_assoc i mapping 0) (circuit_outputs c);
+    circuit_outputs := List.map (fun i => binnat_list_assoc i mapping 0%N) (circuit_outputs c);
   |}.
 
-Register circuit_simplify as vcpu.circuit.simplify.*)
-
-(*Inductive binding :=
-  | binding_Zero
-  | binding_Input (i : nat)
-  | binding_Nand (i j : nat).
-
-Register binding as vcpu.binding.type.
-Register binding_Zero as vcpu.binding.Zero.
-Register binding_Input as vcpu.binding.Input.
-Register binding_Nand as vcpu.binding.Nand.
-
-Record circuit := {
-  circuit_input_count : nat;
-  circuit_wires : list binding;
-  circuit_outputs : list nat;
-  circuit_wires_wf :
-    list_forall_i (fun i b =>
-      match b with
-      | binding_Zero => True
-      | binding_Input j => j < circuit_input_count
-      | binding_Nand j k => j < i /\ k < i
-      end
-    ) circuit_wires;
-  circuit_outputs_wf :
-    list_forall (fun i => i < length circuit_wires) circuit_outputs;
-}.
-
-Register circuit as vcpu.circuit.type.
-Register Build_circuit as vcpu.circuit.constructor.
-Register circuit_input_count as vcpu.circuit.input_count.
-Register circuit_wires as vcpu.circuit.wires.
-Register circuit_outputs as vcpu.circuit.outputs.
-Register circuit_wires_wf as vcpu.circuit.wires_wf.
-Register circuit_outputs_wf as vcpu.circuit.outputs_wf.
-
-Definition circuit_compute_wires_aux start_wire_values wires inputs :=
-  List.fold_left (fun wire_values b =>
-    wire_values ++ [match b with
-    | binding_Zero => false
-    | binding_Input i => List.nth i inputs false
-    | binding_Nand i j =>
-      nandb
-        (List.nth i (start_wire_values ++ wire_values) false)
-        (List.nth j (start_wire_values ++ wire_values) false)
-    end]
-  ) wires [].
-
-Definition circuit_compute_wires c inputs :=
-  circuit_compute_wires_aux [] (circuit_wires c) inputs.
-
-Definition circuit_compute c inputs :=
-  list_select (circuit_compute_wires c inputs) (circuit_outputs c) false.
-
-Theorem length_circuit_compute_wires_aux :
-  forall start_wire_values wires inputs,
-  length (circuit_compute_wires_aux start_wire_values wires inputs) = length wires.
-Proof.
-  cut (forall start_wire_values wires inputs init_wire_values, length (List.fold_left (fun wire_values b =>
-      wire_values ++ [match b with
-      | binding_Zero => false
-      | binding_Input i => List.nth i inputs false
-      | binding_Nand i j =>
-        nandb
-          (List.nth i (start_wire_values ++ wire_values) false)
-          (List.nth j (start_wire_values ++ wire_values) false)
-      end]
-    ) wires init_wire_values) = length init_wire_values + length wires).
-  - intros H. intros start_wire_values wires inputs. apply (H _ _ _ []).
-  - intros start_wire_values wires inputs. induction wires as [ | b wires' IH]; intros init_wire_values.
-    + simpl. rewrite PeanoNat.Nat.add_0_r. auto.
-    + simpl. rewrite IH. rewrite List.app_length. simpl. rewrite <- PeanoNat.Nat.add_assoc. auto.
-Qed.
-
-Theorem length_circuit_compute_wires :
-  forall c inputs,
-  length (circuit_compute_wires c inputs) = length (circuit_wires c).
-Proof.
-  intros c inputs. unfold circuit_compute_wires. apply length_circuit_compute_wires_aux.
-Qed.
-
-Theorem circuit_compute_wires_aux_app :
-  forall start_wire_values wires_1 wires_2 inputs,
-  circuit_compute_wires_aux start_wire_values (wires_1 ++ wires_2) inputs =
-    let wire_values_1 := circuit_compute_wires_aux start_wire_values wires_1 inputs in
-    wire_values_1 ++ circuit_compute_wires_aux (start_wire_values ++ wire_values_1) wires_2 inputs.
-Proof.
-  intros start_wire_values wires_1 wires_2 inputs. simpl. unfold circuit_compute_wires_aux.
-  rewrite List.fold_left_app. rewrite list_fold_left_app_shift. f_equal. apply list_fold_left_ext.
-  intros wire_values b. destruct b as [ | j | j k]; do 2 f_equal. f_equal.
-  - f_equal. apply List.app_assoc.
-  - f_equal. apply List.app_assoc.
-Qed.
-
-Definition circuit_set_outputs c outputs (H : list_forall (fun i => i < length (circuit_wires c)) outputs) := {|
-  circuit_input_count := circuit_input_count c;
-  circuit_wires := circuit_wires c;
-  circuit_outputs := outputs;
-  circuit_wires_wf := circuit_wires_wf c;
-  circuit_outputs_wf := H;
-|}.
-
-Register circuit_set_outputs as vcpu.circuit.set_outputs.
-
-#[program] Definition circuit_empty input_count := {|
-  circuit_input_count := input_count;
-  circuit_wires := list_init (fun i => binding_Input i) input_count;
-  circuit_outputs := [];
-|}.
-Next Obligation.
-  intros input_count. rewrite list_forall_i_list_init. auto.
-Qed.
-Next Obligation.
-  simpl. auto.
-Qed.
-
-Register circuit_empty as vcpu.circuit.empty.
-
-Lemma circuit_empty_spec_wires :
-  forall input_count,
-  forall inputs, length inputs = input_count ->
-  circuit_compute_wires (circuit_empty input_count) inputs = inputs.
-Proof.
-  intros input_count inputs H. unfold circuit_compute_wires, circuit_compute_wires_aux, circuit_empty. simpl.
-  rewrite list_fold_left_list_init. rewrite <- H; clear input_count H.
-  cut (forall l,
-    List.fold_left (fun y z => y ++ [List.nth z inputs false]) (List.seq 0 (length inputs)) l = l ++ inputs).
-  - intros H. apply H.
-  - induction inputs as [ | x inputs' IH]; intros l.
-    + simpl. apply List.app_nil_end.
-    + simpl. rewrite (list_fold_left_list_seq_shift _ 0 1). rewrite IH. rewrite List.app_assoc_reverse. auto.
-Qed.
-
-Lemma circuit_empty_spec :
-  forall input_count,
-  forall inputs, length inputs = input_count ->
-  circuit_compute (circuit_empty input_count) inputs = [].
-Proof.
-  intros input_count inputs H. unfold circuit_compute, circuit_empty. auto.
-Qed.
-
-#[program] Definition circuit_zero := {|
-  circuit_input_count := 0;
-  circuit_wires := [binding_Zero];
-  circuit_outputs := [0];
-|}.
-Next Obligation.
-  unfold list_forall_i. simpl. lia.
-Qed.
-Next Obligation.
-  simpl. lia.
-Qed.
-
-Register circuit_zero as vcpu.circuit.zero.
-
-Lemma circuit_zero_spec_wires :
-  circuit_compute_wires circuit_zero [] = [false].
-Proof.
-  auto.
-Qed.
-
-Lemma circuit_zero_spec :
-  circuit_compute circuit_zero [] = [false].
-Proof.
-  auto.
-Qed.
-
-#[program] Definition circuit_one := {|
-  circuit_input_count := 0;
-  circuit_wires := [binding_Zero; binding_Nand 0 0];
-  circuit_outputs := [1];
-|}.
-Next Obligation.
-  unfold list_forall_i. simpl. lia.
-Qed.
-Next Obligation.
-  simpl. lia.
-Qed.
-
-Register circuit_one as vcpu.circuit.one.
-
-Lemma circuit_one_spec_wires :
-  circuit_compute_wires circuit_one [] = [false; true].
-Proof.
-  auto.
-Qed.
-
-Lemma circuit_one_spec :
-  circuit_compute circuit_one [] = [true].
-Proof.
-  auto.
-Qed.
-
-#[program] Definition circuit_nand := {|
-  circuit_input_count := 2;
-  circuit_wires := [binding_Input 0; binding_Input 1; binding_Nand 0 1];
-  circuit_outputs := [2];
-|}.
-Next Obligation.
-  unfold list_forall_i. simpl. lia.
-Qed.
-Next Obligation.
-  simpl. lia.
-Qed.
-
-Lemma circuit_nand_spec_wires :
-  forall i j,
-  circuit_compute_wires circuit_nand [i; j] = [i; j; nandb i j].
-Proof.
-  auto.
-Qed.
-
-Lemma circuit_nand_spec :
-  forall i j,
-  circuit_compute circuit_nand [i; j] = [nandb i j].
-Proof.
-  auto.
-Qed.
-
-Unset Program Cases.
-
-#[program] Definition circuit_add c_parent c_child input_wires
-  (H1 : length input_wires = circuit_input_count c_child)
-  (H2 : list_forall (fun i => i < length (circuit_wires c_parent)) input_wires) := {|
-  circuit_input_count := circuit_input_count c_parent;
-  circuit_wires :=
-    circuit_wires c_parent ++
-    List.map (fun i => binding_Nand i i) input_wires ++
-    List.map (fun b =>
-      match b with
-      | binding_Zero => binding_Zero
-      | binding_Input i =>
-        binding_Nand (length (circuit_wires c_parent) + i) (length (circuit_wires c_parent) + i)
-      | binding_Nand i j =>
-        binding_Nand
-          (length (circuit_wires c_parent) + circuit_input_count c_child + i)
-          (length (circuit_wires c_parent) + circuit_input_count c_child + j)
-      end
-    ) (circuit_wires c_child);
-  circuit_outputs := circuit_outputs c_parent;
-|}.
-Next Obligation.
-  intros c_parent c_child input_wires H1 H2. rewrite list_forall_i_app; split.
-  - apply (circuit_wires_wf c_parent).
-  - rewrite list_forall_i_aux_app; split.
-    + rewrite list_forall_i_aux_map. rewrite list_forall_i_aux_equiv.
-      rewrite list_forall_list_forall_i in H2. apply (list_forall_i_incr _ _ _ H2). lia.
-    + rewrite list_forall_i_aux_map. rewrite List.map_length.
-      cut (
-        list_forall_i_aux (fun i b =>
-          match b with
-          | binding_Zero => True
-          | binding_Input j =>
-            length (circuit_wires c_parent) + j < i /\ length (circuit_wires c_parent) + j < i
-          | binding_Nand j k =>
-            length (circuit_wires c_parent) + circuit_input_count c_child + j < i /\
-            length (circuit_wires c_parent) + circuit_input_count c_child + k < i
-          end
-        ) (length (circuit_wires c_parent) + length input_wires) (circuit_wires c_child)
-      ).
-      * intros H. apply (list_forall_i_aux_incr _ _ _ _ H). intros i b. destruct b; auto.
-      * rewrite list_forall_i_aux_equiv. apply (list_forall_i_incr _ _ _ (circuit_wires_wf c_child)).
-        intros i b. destruct b; lia.
-Qed.
-Next Obligation.
-  intros c_parent c_child input_wires H1 H2. apply (list_forall_incr _ _ _ (circuit_outputs_wf c_parent)).
-  rewrite List.app_length. lia.
-Qed.
-
-Set Program Cases.
-
-Register circuit_add as vcpu.circuit.add.
-
-Lemma circuit_add_spec_wires :
-  forall c_parent c_child input_wires
-  (H1 : length input_wires = circuit_input_count c_child)
-  (H2 : list_forall (fun i => i < length (circuit_wires c_parent)) input_wires),
-  forall inputs, length inputs = circuit_input_count c_parent ->
-  let c_parent_wire_values := circuit_compute_wires c_parent inputs in
-  let c_child_inputs := list_select c_parent_wire_values input_wires false in
-  circuit_compute_wires (circuit_add c_parent c_child input_wires H1 H2) inputs =
-    c_parent_wire_values ++
-    List.map negb c_child_inputs ++
-    circuit_compute_wires c_child c_child_inputs.
-Proof.
-  intros c_parent c_child input_wires H1 H2. intros inputs H3. intros c_parent_wire_values c_child_inputs.
-  unfold circuit_compute_wires, circuit_add. simpl. rewrite circuit_compute_wires_aux_app. simpl.
-  replace (circuit_compute_wires_aux [] (circuit_wires c_parent) inputs) with c_parent_wire_values by auto.
-  rewrite circuit_compute_wires_aux_app. simpl. f_equal.
-  assert (HA : circuit_compute_wires_aux c_parent_wire_values
-    (List.map (fun i => binding_Nand i i) input_wires) inputs = List.map negb c_child_inputs). {
-    subst c_child_inputs. unfold circuit_compute_wires_aux, list_select. rewrite list_fold_left_list_map.
-    rewrite List.map_map. rewrite (list_fold_left_ext_precise _ (fun wire_values i =>
-      wire_values ++ [negb (List.nth i c_parent_wire_values false)])).
-    - apply (eq_sym (list_map_list_fold_left _ _)).
-    - intros y. apply (list_forall_incr _ _ _ H2). intros z H. rewrite nandb_negb. do 3 f_equal.
-      apply List.app_nth1. subst c_parent_wire_values. rewrite length_circuit_compute_wires. auto.
-  }
-  f_equal.
-  - auto.
-  - rewrite HA; clear HA. unfold circuit_compute_wires_aux at 1. rewrite list_fold_left_list_map.
-    rewrite (list_fold_left_ext _
-      (fun wire_values b =>
-       wire_values ++
-       [match b with
-        | binding_Zero => false
-        | binding_Input i =>
-          nandb
-            (List.nth (length (circuit_wires c_parent) + i)
-              ((c_parent_wire_values ++ List.map negb c_child_inputs) ++ wire_values) false)
-            (List.nth (length (circuit_wires c_parent) + i)
-              ((c_parent_wire_values ++ List.map negb c_child_inputs) ++ wire_values) false)
-        | binding_Nand i j =>
-          nandb
-            (List.nth (length (circuit_wires c_parent) + circuit_input_count c_child + i)
-              ((c_parent_wire_values ++ List.map negb c_child_inputs) ++ wire_values) false)
-            (List.nth (length (circuit_wires c_parent) + circuit_input_count c_child + j)
-              ((c_parent_wire_values ++ List.map negb c_child_inputs) ++ wire_values) false)
-        end])
-    ).
-    + rewrite (list_fold_left_ext_precise _
-      (fun wire_values b =>
-         wire_values ++
-         [match b with
-          | binding_Zero => false
-          | binding_Input i => negb (List.nth i (List.map negb c_child_inputs) false)
-          | binding_Nand i j => nandb (List.nth i wire_values false) (List.nth j wire_values false)
-          end])
-      ).
-      * unfold circuit_compute_wires_aux. apply list_fold_left_ext_precise.
-        intros wire_values. rewrite list_forall_list_forall_i.
-        apply (list_forall_i_incr _ _ _ (circuit_wires_wf c_child)). intros i b H.
-        destruct b as [ | j | j k]; simpl; do 2 f_equal. rewrite <- Bool.negb_involutive. f_equal.
-        rewrite <- (List.map_nth negb). apply List.nth_indep.
-        rewrite List.map_length. subst c_child_inputs. rewrite length_list_select. lia.
-      * intros wire_values. rewrite list_forall_list_forall_i.
-        apply (list_forall_i_incr _ _ _ (circuit_wires_wf c_child)). intros i b H.
-        destruct b as [ | j | j k]; simpl; do 2 f_equal.
-        -- rewrite nandb_negb. f_equal. rewrite List.app_nth1.
-           ++ rewrite List.app_nth2.
-              ** f_equal. subst c_parent_wire_values. rewrite length_circuit_compute_wires. lia.
-              ** subst c_parent_wire_values. rewrite length_circuit_compute_wires. lia.
-           ++ rewrite List.app_length. subst c_parent_wire_values. rewrite length_circuit_compute_wires.
-              rewrite List.map_length. subst c_child_inputs. rewrite length_list_select. lia.
-        -- f_equal.
-           ++ rewrite List.app_nth2.
-              ** rewrite List.app_length. f_equal.
-                 subst c_parent_wire_values. rewrite length_circuit_compute_wires.
-                 rewrite List.map_length. subst c_child_inputs. rewrite length_list_select.
-                 lia.
-              ** rewrite List.app_length.
-                 subst c_parent_wire_values. rewrite length_circuit_compute_wires.
-                 rewrite List.map_length. subst c_child_inputs. rewrite length_list_select.
-                 lia.
-            ++ rewrite List.app_nth2.
-              ** rewrite List.app_length. f_equal.
-                 subst c_parent_wire_values. rewrite length_circuit_compute_wires.
-                 rewrite List.map_length. subst c_child_inputs. rewrite length_list_select.
-                 lia.
-              ** rewrite List.app_length.
-                 subst c_parent_wire_values. rewrite length_circuit_compute_wires.
-                 rewrite List.map_length. subst c_child_inputs. rewrite length_list_select.
-                 lia.
-    + intros wire_values b. destruct b; auto.
-Qed.
-
-Definition circuit_add_parent_wires c_parent c_child input_wires
-  (H1 : length input_wires = circuit_input_count c_child)
-  (H2 : list_forall (fun i => i < length (circuit_wires c_parent)) input_wires) :=
-  List.seq 0 (length (circuit_wires c_parent)).
-
-Definition circuit_add_child_wires c_parent c_child input_wires
-  (H1 : length input_wires = circuit_input_count c_child)
-  (H2 : list_forall (fun i => i < length (circuit_wires c_parent)) input_wires) :=
-  List.seq (length (circuit_wires c_parent) + circuit_input_count c_child) (length (circuit_wires c_child)).
-
-Definition circuit_add_child_output_wires c_parent c_child input_wires
-  (H1 : length input_wires = circuit_input_count c_child)
-  (H2 : list_forall (fun i => i < length (circuit_wires c_parent)) input_wires) :=
-  list_select (circuit_add_child_wires c_parent c_child input_wires H1 H2) (circuit_outputs c_child) 0.
-
-Register circuit_add_child_output_wires as vcpu.circuit.add_child_output_wires.
-
-Lemma circuit_add_spec_parent_wires :
-  forall c_parent c_child input_wires
-  (H1 : length input_wires = circuit_input_count c_child)
-  (H2 : list_forall (fun i => i < length (circuit_wires c_parent)) input_wires),
-  forall inputs, length inputs = circuit_input_count c_parent ->
-  list_select (circuit_compute_wires (circuit_add c_parent c_child input_wires H1 H2) inputs)
-    (circuit_add_parent_wires c_parent c_child input_wires H1 H2) false =
-    circuit_compute_wires c_parent inputs.
-Proof.
-  intros c_parent c_child input_wires H1 H2. intros inputs H3. rewrite (circuit_add_spec_wires _ _ _ _ _ _ H3).
-  unfold circuit_add_parent_wires.
-  replace (List.seq 0 (length (circuit_wires c_parent)))
-    with (List.seq 0 (length (circuit_compute_wires c_parent inputs))).
-  - apply list_select_app_1_seq.
-  - f_equal. apply length_circuit_compute_wires.
-Qed.
-
-Lemma circuit_add_spec_child_wires :
-  forall c_parent c_child input_wires
-  (H1 : length input_wires = circuit_input_count c_child)
-  (H2 : list_forall (fun i => i < length (circuit_wires c_parent)) input_wires),
-  forall inputs, length inputs = circuit_input_count c_parent ->
-  list_select (circuit_compute_wires (circuit_add c_parent c_child input_wires H1 H2) inputs)
-    (circuit_add_child_wires c_parent c_child input_wires H1 H2) false =
-    circuit_compute_wires c_child (list_select (circuit_compute_wires c_parent inputs) input_wires false).
-Proof.
-  intros c_parent c_child input_wires H1 H2. intros inputs H3. rewrite (circuit_add_spec_wires _ _ _ _ _ _ H3).
-  unfold circuit_add_child_wires. rewrite List.app_assoc.
-  replace (List.seq (length (circuit_wires c_parent) + circuit_input_count c_child)
-      (length (circuit_wires c_child)))
-    with (List.seq (length (circuit_compute_wires c_parent inputs ++
-      List.map negb (list_select (circuit_compute_wires c_parent inputs) input_wires false)))
-      (length (circuit_compute_wires c_child (list_select (circuit_compute_wires c_parent inputs)
-      input_wires false)))).
-  - apply list_select_app_2_seq.
-  - f_equal.
-    + rewrite List.app_length. f_equal.
-      * apply length_circuit_compute_wires.
-      * rewrite List.map_length. rewrite length_list_select. auto.
-    + apply length_circuit_compute_wires.
-Qed.
-
-Lemma circuit_add_spec_child_output_wires :
-  forall c_parent c_child input_wires
-  (H1 : length input_wires = circuit_input_count c_child)
-  (H2 : list_forall (fun i => i < length (circuit_wires c_parent)) input_wires),
-  forall inputs, length inputs = circuit_input_count c_parent ->
-  list_select (circuit_compute_wires (circuit_add c_parent c_child input_wires H1 H2) inputs)
-    (circuit_add_child_output_wires c_parent c_child input_wires H1 H2) false =
-    circuit_compute c_child (list_select (circuit_compute_wires c_parent inputs) input_wires false).
-Proof.
-  intros c_parent c_child input_wires H1 H2. intros inputs H3.
-  unfold circuit_compute. rewrite <- (circuit_add_spec_child_wires _ _ _ H1 H2 _ H3).
-  unfold circuit_add_child_output_wires. apply list_select_com.
-  apply (list_forall_incr _ _ _ (circuit_outputs_wf c_child)). intros i H4.
-  unfold circuit_add_child_wires. rewrite List.seq_length. auto.
-Qed.
-
-#[program] Definition circuit_add_fast c_parent c_child input_wires
-  (H1 : length input_wires = circuit_input_count c_child)
-  (H2 : list_forall (fun i => i < length (circuit_wires c_parent)) input_wires) := {|
-  circuit_input_count := circuit_input_count c_parent;
-  circuit_wires :=
-    circuit_wires c_parent ++
-    List.map (fun b =>
-      match b with
-      | binding_Zero => binding_Zero
-      | binding_Input i =>
-        List.nth (List.nth i input_wires 0) (circuit_wires c_parent) binding_Zero
-      | binding_Nand i j =>
-        binding_Nand (length (circuit_wires c_parent) + i) (length (circuit_wires c_parent) + j)
-      end
-    ) (circuit_wires c_child);
-  circuit_outputs := circuit_outputs c_parent;
-|}.
-Next Obligation.
-  intros c_parent c_child input_wires H1 H2. rewrite list_forall_i_app; split.
-  - apply (circuit_wires_wf c_parent).
-  - rewrite list_forall_i_aux_map. rewrite list_forall_i_aux_equiv.
-Admitted.
-Next Obligation.
-Admitted.
-
-Register circuit_add_fast as vcpu.circuit.add_fast.
-
-#[program] Definition circuit_switch data_size := {|
-  circuit_input_count := 1 + 2 * data_size;
-  circuit_wires :=
-    list_init (fun i => binding_Input i) (1 + 2 * data_size) ++
-    binding_Nand 0 0 ::
-    list_init (fun i => binding_Nand (1 + 2 * data_size) (1 + i)) data_size ++
-    list_init (fun i => binding_Nand 0 (1 + data_size + i)) data_size ++
-    list_init (fun i => binding_Nand (2 + 2 * data_size + i) (2 + 3 * data_size + i)) data_size;
-  circuit_outputs := List.seq (2 + 4 * data_size) data_size;
-|}.
-Next Obligation.
-  intros data_size. rewrite list_forall_i_app; split.
-  - rewrite list_forall_i_list_init. auto.
-  - simpl; split.
-    + lia.
-    + rewrite list_forall_i_aux_app; split.
-      * rewrite list_forall_i_aux_equiv. rewrite list_forall_i_list_init.
-        intros i H. rewrite length_list_init_aux. lia.
-      * rewrite list_forall_i_aux_app; split.
-        -- rewrite list_forall_i_aux_equiv. rewrite list_forall_i_list_init.
-           intros i H. rewrite length_list_init_aux. lia.
-        -- rewrite list_forall_i_aux_equiv. rewrite list_forall_i_list_init.
-           intros i H. rewrite length_list_init_aux, ? length_list_init. lia.
-Qed.
-Next Obligation.
-  intros data_size. rewrite list_forall_list_seq. rewrite List.app_length. simpl.
-  rewrite ? List.app_length. rewrite length_list_init_aux, ? length_list_init. lia.
-Qed.
-
-Register circuit_switch as vcpu.circuit.switch.
-
-Lemma circuit_switch_spec_wires :
-  forall data_size,
-  forall inputs, length inputs = 1 + 2 * data_size ->
-  circuit_compute_wires (circuit_switch data_size) inputs =
-    inputs ++
-    negb (List.nth 0 inputs false) ::
-    List.map (fun b => nandb (negb (List.nth 0 inputs false)) b)
-      (list_select inputs (List.seq 1 data_size) false) ++
-    List.map (fun b => nandb (List.nth 0 inputs false) b)
-      (list_select inputs (List.seq (1 + data_size) data_size) false) ++
-    if List.nth 0 inputs false
-    then list_select inputs (List.seq (1 + data_size) data_size) false
-    else list_select inputs (List.seq 1 data_size) false.
-Proof.
-  intros data_size. intros inputs H1. unfold circuit_compute_wires, circuit_switch. cbv [circuit_wires].
-  rewrite circuit_compute_wires_aux_app. simpl. f_equal.
-  - apply (circuit_empty_spec_wires (1 + 2 * data_size) inputs H1).
-  - specialize (circuit_empty_spec_wires (1 + 2 * data_size) inputs H1) as H2.
-    unfold circuit_compute_wires, circuit_empty in H2. simpl in H2. rewrite H2. clear H2.
-    rewrite <- list_cons_app. rewrite circuit_compute_wires_aux_app.
-    assert (A1 : circuit_compute_wires_aux inputs [binding_Nand 0 0] inputs =
-        [negb (List.nth 0 inputs false)]). {
-      cbn. rewrite nandb_negb. rewrite List.app_nil_r. auto.
-    }
-    rewrite A1. simpl. f_equal. destruct inputs as [ | b inputs'].
-    + simpl in H1. congruence.
-    + simpl in H1. injection H1 as H1. simpl. rewrite circuit_compute_wires_aux_app. simpl.
-      assert (A2 : circuit_compute_wires_aux (b :: inputs' ++ [negb b])
-          (list_init (fun i => binding_Nand (S (data_size + (data_size + 0))) (S i)) data_size) 
-          (b :: inputs') =
-          List.map (fun b' => nandb (negb b) b') (list_select (b :: inputs') (List.seq 1 data_size) false)). {
-        unfold circuit_compute_wires_aux. rewrite list_fold_left_list_init.
-        rewrite list_fold_left_ext_precise with (f2 := fun wire_values i =>
-          wire_values ++ [nandb (negb b) (List.nth i inputs' false)]).
-        - rewrite <- list_fold_left_list_init. rewrite list_init_list_map_list_seq.
-          rewrite <- (List.map_map _ (fun x => [x])). rewrite list_fold_left_app_list_map_singleton.
-          unfold list_select. rewrite List.map_map. rewrite <- List.seq_shift. rewrite List.map_map.
-          simpl. auto.
-        - intros wire_values. rewrite list_forall_list_seq. intros i H2. do 3 f_equal.
-           + rewrite List.app_nth1.
-              * simpl. rewrite List.app_nth2.
-                -- rewrite H1. rewrite PeanoNat.Nat.sub_diag. auto.
-                -- lia.
-              * simpl. rewrite List.app_length. simpl. lia.
-           + simpl. rewrite <- List.app_assoc. apply List.app_nth1. lia.
-      }
-      rewrite ? A2. f_equal. rewrite ? List.app_comm_cons. rewrite circuit_compute_wires_aux_app. simpl.
-      assert (A3 : circuit_compute_wires_aux
-          (b :: (inputs' ++ [negb b]) ++
-             List.map (fun b' => nandb (negb b) b') (list_select (b :: inputs') (List.seq 1 data_size) false))
-          (list_init (fun i : nat => binding_Nand 0 (S (data_size + i))) data_size) (b :: inputs') =
-          List.map (fun b' => nandb b b') (list_select (b :: inputs')
-            (List.seq (S data_size) data_size) false)). {
-        admit.
-      }
-      rewrite ? A3. f_equal. destruct b.
-      * unfold nandb. simpl. unfold circuit_compute_wires_aux. rewrite list_fold_left_list_init.
-        simpl. admit.
-      * admit.
-Admitted.
-
-Lemma circuit_switch_spec :
-  forall data_size,
-  forall inputs, length inputs = 1 + 2 * data_size ->
-  circuit_compute (circuit_switch data_size) inputs =
-    if List.nth 0 inputs false
-    then list_select inputs (List.seq (1 + data_size) data_size) false
-    else list_select inputs (List.seq 1 data_size) false.
-Proof.
-  intros data_size. intros inputs H1. unfold circuit_compute. rewrite (circuit_switch_spec_wires _ _ H1).
-  rewrite <- list_cons_app. rewrite ? List.app_assoc. simpl.
-  assert (A1 : List.length (((inputs ++ [negb (List.nth 0 inputs false)]) ++
-      List.map (fun b : bool => nandb (negb (List.nth 0 inputs false)) b)
-        (list_select inputs (List.seq 1 data_size) false)) ++
-      List.map (fun b : bool => nandb (List.nth 0 inputs false) b)
-        (list_select inputs (List.seq (S data_size) data_size) false)) =
-        S (S (data_size + (data_size + (data_size + (data_size + 0)))))). {
-    rewrite ? List.app_length. rewrite H1. rewrite ? List.map_length. rewrite ? length_list_select.
-    rewrite ? List.seq_length. simpl. lia.
-  }
-  assert (A2 : List.length (if List.nth 0 inputs false
-      then list_select inputs (List.seq (S data_size) data_size) false
-      else list_select inputs (List.seq 1 data_size) false) =
-      data_size). {
-    destruct (List.nth 0 inputs false); rewrite length_list_select; apply List.seq_length.
-  }
-  rewrite <- A2 at 11. rewrite <- A1. apply list_select_app_2_seq.
-Qed.
-*)
+Register circuit_simplify as vcpu.circuit.simplify.
